theories/RASimpl.v
@@ -1,0 +1,71 @@
+From Prototype Require Import Prelude Sig LevelOne LevelTwo LevelTwoSimp LevelTwoClean.
+From Ltac2 Require Import RedFlags Printf.
+
+(*********************************************************************************)
+(** *** Load the plugin. *)
+(*********************************************************************************)
+
+Declare ML Module "autosubst-experiments.plugin".
+
+Ltac2 @external reify_term : constr -> constr * constr := "autosubst-experiments.plugin" "reify_term".
+Ltac2 @external reify_subst : constr -> constr * constr := "autosubst-experiments.plugin" "reify_subst".
+Ltac2 @external eval_term : constr -> constr * constr := "autosubst-experiments.plugin" "eval_term".
+Ltac2 @external eval_subst : constr -> constr * constr := "autosubst-experiments.plugin" "eval_subst".
+
+(*********************************************************************************)
+(** *** Instantiate the generic level 1 and level 2 machinery. *)
+(*********************************************************************************)
+
+(** [Make (S)] creates modules: 
+    - [T] with level two expressions/substitutions built on signature [S].
+    - [O] with level one expressions/substitutions built on signature [S]. *)
+Module Make (S : Sig).
+Include LevelTwoClean.Make (S).
+
+(** Reduction flags to unfold all simplification functions (LevelTwoSimp.v). *)
+Ltac2 red_flags_simp () : RedFlags.t := 
+  red_flags:(beta iota delta 
+    [esimp ssimp esimp_functional ssimp_functional
+     qsimp rsimp qsimp_functional rsimp_functional
+     substitute scomp substitute_functional scomp_functional
+     rename srcomp rename_functional srcomp_functional
+     tnat sren tnat_functional sren_functional
+     substitute_aux scomp_aux sapply_aux sup rup 
+     sapply rscomp sapply_functional rscomp_functional
+     rapply rcomp rapply_functional rcomp_functional
+     rcomp_aux rapply_aux rcons scons]).
+
+(** Reduction flags to unfold all cleanup functions (LevelTwoClean.v). *)
+Ltac2 red_flags_clean () : RedFlags.t :=
+  red_flags:(beta iota delta 
+    [eclean sclean eclean_functional sclean_functional
+     qclean rclean qclean_functional rclean_functional
+     eclean_ren eclean_subst eclean_subst_clause_1
+     qclean_rapply qclean_rapply_clause_1
+     dest_rshift dest_rshift_clause_2 dest_rshift_clause_2_clause_1
+     mk_qsucc dest_var
+     dest_ren dest_ren_clause_3 dest_ren_clause_3_clause_1 
+     dest_ren_clause_4 dest_ren_clause_4_clause_1
+     ]).
+
+(** Reduction flags to unfold all (level 2 -> level 1) evaluation 
+    functions (LevelTwo.v). *)
+Ltac2 red_flags_eval () : RedFlags.t :=
+  red_flags:(beta iota delta   
+    [eeval seval eeval_functional seval_functional
+     reval qeval reval_functional qeval_functional
+     assign_qnat assign_ren assign_term assign_subst
+     List.nth (* TODO use something else than [Lisnth]. *)
+     ]).
+
+End Make.
+
+(*********************************************************************************)
+(** *** [rasimpl]. *)
+(*********************************************************************************)
+
+(** [Simplification x y] expresses the fact that [x] simplifies into [y].
+    Typically [x] is a ground term and [y] is an evar, and a proof of 
+    [Simplification x y] instantiates [y] with a simplified version of [x]. *)
+Class Simplification T (x y : T) := 
+  MkSimplification { simplification : x = y }.
